compiler/backend/proofs/bvl_to_bviProofScript.sml
@@ -68,6 +68,7 @@ val state_rel_def = Define `
     (s.clock = t.clock) /\
     (lookup AllocGlobal_location t.code = SOME AllocGlobal_code) ∧
     (lookup CopyGlobals_location t.code = SOME CopyGlobals_code) ∧
+    (lookup ListLength_location t.code = SOME ListLength_code) ∧
     (* (lookup InitGlobals_location t.code = SOME InitGlobals_code start) ∧ *)
     (!name arity exp.
        (lookup name s.code = SOME (arity,exp)) ==>
@@ -420,7 +421,7 @@ val evaluate_AllocGlobal_code = Q.prove(
     simp[Abbr`rf`,FLOOKUP_UPDATE] >>
     IF_CASES_TAC >> simp[] >- (
       full_simp_tac(srw_ss())[FLOOKUP_DEF] >> metis_tac[LEAST_NOTIN_FDOM] ) >>
-    simp[Abbr`l1`,LENGTH_REPLICATE] ) >>
+    simp[Abbr`l1`,LENGTH_REPLICATE] \\ intLib.COOPER_TAC ) >>
   strip_tac >>
   qexists_tac`c+1` >>
   simp[] >>
@@ -434,7 +435,38 @@ val evaluate_AllocGlobal_code = Q.prove(
   srw_tac[][] >> simp[] >> TRY(intLib.COOPER_TAC) >>
   `n = LENGTH ls`by decide_tac >>
   `2 * (LENGTH ls + 1) = LENGTH ls + LENGTH ls + 2` by DECIDE_TAC >>
-  simp[Abbr`l1`,DROP_REPLICATE,ADD1])
+  simp[Abbr`l1`,DROP_REPLICATE,ADD1]
+  \\ AP_THM_TAC \\ AP_TERM_TAC
+  \\ intLib.COOPER_TAC)
+
+val evaluate_ListLength_code = store_thm("evaluate_ListLength_code",
+  ``!lv vs n.
+      lookup ListLength_location s.code = SOME (2,SND ListLength_code) /\
+      v_to_list lv = SOME vs ==>
+      ∃p1 c.
+        evaluate ([SND ListLength_code],[lv;Number (&n)],inc_clock c s) =
+          (Rval [Number (&(n + LENGTH vs))],s)``,
+  HO_MATCH_MP_TAC v_to_list_ind \\ rw [] \\ fs [v_to_list_def] \\ rveq
+  \\ fs [ListLength_code_def] THEN1
+   (fs [bviSemTheory.evaluate_def,EVAL ``Boolv T``,
+        EVAL ``bviSem$do_app (TagLenEq nil_tag 0) [Block nil_tag []] s``]
+    \\ fs [inc_clock_def,bviSemTheory.state_component_equality])
+  \\ simp [bviSemTheory.evaluate_def,EVAL ``Boolv T``]
+  \\ fs [EVAL ``bviSem$do_app (TagLenEq nil_tag 0) [Block cons_tag [h; lv]] s``,
+         EVAL ``bviSem$do_app (Const 1) [] s``,
+         EVAL ``bviSem$do_app (Const 0) [] s``,EVAL ``Boolv F``,
+         EVAL ``bviSem$do_app El [Block cons_tag [h; lv]; Number 1] s``,
+         EVAL ``bviSem$do_app Add [Number (&n); Number (&m)] s``,
+         bvlSemTheory.find_code_def]
+  \\ Cases_on `v_to_list lv` \\ fs [] \\ rw [] \\ fs []
+  \\ first_x_assum (qspec_then `n+1` mp_tac) \\ strip_tac
+  \\ qexists_tac `c+1` \\ fs []
+  \\ qpat_abbrev_tac `s1 = dec_clock 1 _`
+  \\ `inc_clock c s = s1` by
+   (unabbrev_all_tac \\ fs [bviSemTheory.state_component_equality,
+       bviSemTheory.dec_clock_def])
+  \\ fs [] \\ pop_assum kall_tac
+  \\ `(1 + &n) = (&(n + 1))` by intLib.COOPER_TAC \\ fs []);
 
 (* compiler correctness *)
 
@@ -514,11 +546,24 @@ val iEval_bVarBound = Q.prove(
     \\ FIRST_X_ASSUM (MP_TAC o Q.SPECL [`n`,`vs`]) \\ full_simp_tac(srw_ss())[]
     \\ full_simp_tac(srw_ss())[iEval_def] \\ NO_TAC)
   THEN1
-   (FIRST_X_ASSUM (MP_TAC o Q.SPECL [`n`,`vs`]) \\ full_simp_tac(srw_ss())[]
-    \\ Cases_on `op` \\ full_simp_tac(srw_ss())[compile_op_def,iEval_def,compile_int_thm]
+   (Cases_on `?t. op = FromList t` THEN1
+     (fs [] \\ rveq \\ fs [compile_op_def]
+      \\ once_rewrite_tac [bviSemTheory.evaluate_def]
+      \\ IF_CASES_TAC THEN1
+        (fs [bviSemTheory.evaluate_def,EVAL ``bviSem$do_app (Const 0) [] s``])
+      \\ FIRST_X_ASSUM (MP_TAC o Q.SPECL [`n`,`vs`])
+      \\ full_simp_tac(srw_ss())[]
+      \\ CASE_TAC \\ fs [] \\ CASE_TAC \\ fs []
+      \\ imp_res_tac evaluate_IMP_LENGTH
+      \\ Cases_on `a` \\ fs [LENGTH_NIL]
+      \\ fs [bviSemTheory.evaluate_def])
+    \\ FIRST_X_ASSUM (MP_TAC o Q.SPECL [`n`,`vs`]) \\ full_simp_tac(srw_ss())[]
+    \\ Cases_on `op`
+    \\ full_simp_tac(srw_ss())[compile_op_def,iEval_def,compile_int_thm]
     \\ simp[iEval_def]
     \\ simp[iEval_append,iEval_def,compile_int_thm]
-    \\ BasicProvers.EVERY_CASE_TAC \\ full_simp_tac(srw_ss())[iEval_def,compile_int_thm])
+    \\ BasicProvers.EVERY_CASE_TAC
+    \\ full_simp_tac(srw_ss())[iEval_def,compile_int_thm])
   \\ full_simp_tac(srw_ss())[iEval_def]
   \\ FIRST_X_ASSUM (MP_TAC o Q.SPECL [`n2`]) \\ full_simp_tac(srw_ss())[]
   \\ FIRST_X_ASSUM (MP_TAC o Q.SPECL [`n`,`vs`]) \\ full_simp_tac(srw_ss())[]
@@ -635,8 +680,8 @@ val do_app_adjust = Q.prove(
       metis_tac[INJ_DEF]) >>
     METIS_TAC[])
   THEN1 (* FromList *) (
-    Cases_on`REVERSE a`>>full_simp_tac(srw_ss())[]>>
-    Cases_on`t`>>full_simp_tac(srw_ss())[] >>
+    Cases_on `REVERSE a` \\ fs [] \\ Cases_on `t` \\ fs []
+    \\ fs [bvlSemTheory.do_app_def] >>
     simp[bEvalOp_def,v_to_list_adjust] >>
     Cases_on`v_to_list h`>>simp[] >> strip_tac >>
     rpt var_eq_tac >> simp[bvl_to_bvi_id,adjust_bv_def] >>
@@ -1241,17 +1286,24 @@ val compile_exps_correct = Q.prove(
       \\ full_simp_tac(srw_ss())[EVERY_MEM] \\ RES_TAC))
   THEN1 (* Op *)
    (`?c1 aux1 n1. compile_exps n xs = (c1,aux1,n1)` by METIS_TAC [PAIR]
-    \\ full_simp_tac(srw_ss())[LET_DEF] \\ SRW_TAC [] [] \\ full_simp_tac(srw_ss())[PULL_FORALL]
+    \\ full_simp_tac(srw_ss())[LET_DEF] \\ SRW_TAC [] []
+    \\ full_simp_tac(srw_ss())[PULL_FORALL]
     \\ `?res5 s5. evaluate (xs,env,s) = (res5,s5)` by METIS_TAC [PAIR]
-    \\ full_simp_tac(srw_ss())[] \\ FIRST_X_ASSUM (MP_TAC o Q.SPEC `n`) \\ full_simp_tac(srw_ss())[]
+    \\ full_simp_tac(srw_ss())[]
+    \\ FIRST_X_ASSUM (MP_TAC o Q.SPEC `n`) \\ full_simp_tac(srw_ss())[]
     \\ reverse (Cases_on `res5`) \\ full_simp_tac(srw_ss())[] \\ SRW_TAC [] []
-    \\ first_x_assum (MP_TAC o Q.SPECL [`t1`,`b1`]) \\ full_simp_tac(srw_ss())[]
+    \\ fs [] \\ first_x_assum drule \\ fs []
     THEN1 (
-      REPEAT STRIP_TAC \\ IMP_RES_TAC compile_exps_LENGTH \\ full_simp_tac(srw_ss())[iEval_def]
+      REPEAT STRIP_TAC \\ IMP_RES_TAC compile_exps_LENGTH
+      \\ full_simp_tac(srw_ss())[iEval_def]
       \\ Q.LIST_EXISTS_TAC [`t2`,`b2`] \\ full_simp_tac(srw_ss())[]
-      \\ Cases_on `op` \\ full_simp_tac(srw_ss())[compile_op_def,iEval_def,compile_int_thm,iEval_append]
+      \\ Cases_on `op`
+      \\ fs[compile_op_def,iEval_def,compile_int_thm,iEval_append]
       \\ qexists_tac`c`>>simp[]>>
-         every_case_tac \\ full_simp_tac(srw_ss())[iEval_def,compile_int_thm])
+         every_case_tac \\ full_simp_tac(srw_ss())[iEval_def,compile_int_thm]
+      \\ imp_res_tac compile_exps_LENGTH
+      \\ fs [NULL_EQ,LENGTH_NIL]
+      \\ Cases_on `xs` \\ fs [bviSemTheory.evaluate_def])
     \\ REPEAT STRIP_TAC \\ Cases_on `do_app op (REVERSE a) s5` \\ full_simp_tac(srw_ss())[]
     \\ TRY(
       srw_tac[][] >>
@@ -1266,6 +1318,36 @@ val compile_exps_correct = Q.prove(
       \\ Cases_on `REVERSE a` \\ full_simp_tac(srw_ss())[iEval_def,iEvalOp_def]
       \\ full_simp_tac(srw_ss())[EVAL ``do_app_aux (Const 0) [] t2``]
       \\ SRW_TAC [] [adjust_bv_def])
+    \\ Cases_on `?i. op = FromList i` \\ full_simp_tac(srw_ss())[] THEN1
+     (fs [compile_op_def] \\ rveq
+      \\ fs [bvlSemTheory.do_app_def]
+      \\ Cases_on `REVERSE a` \\ fs [] \\ Cases_on `t` \\ fs [] \\ rveq \\ fs []
+      \\ Cases_on `v_to_list h` \\ fs []
+      \\ drule evaluate_IMP_LENGTH \\ rveq
+      \\ Cases_on `c1` \\ fs [LENGTH_NIL]
+      \\ strip_tac \\ rveq \\ fs []
+      \\ qexists_tac `t2`
+      \\ qexists_tac `b2`
+      \\ `lookup ListLength_location t2.code = SOME ListLength_code` by
+              (fs [state_rel_def] \\ NO_TAC) \\ fs []
+      \\ fs [EVAL ``ListLength_code``] \\ fs [GSYM (EVAL ``SND ListLength_code``)]
+      \\ `v_to_list (adjust_bv b2 h) = SOME (MAP (adjust_bv b2) x)` by
+             fs [v_to_list_adjust]
+      \\ drule evaluate_ListLength_code
+      \\ disch_then drule \\ fs []
+      \\ disch_then (qspec_then `0` strip_assume_tac)
+      \\ qexists_tac `c+1+c'`
+      \\ fs [bviSemTheory.evaluate_def,EVAL ``bviSem$do_app (Const 0) [] t2``]
+      \\ qpat_assum `evaluate ([h'],_) = _` assume_tac
+      \\ drule evaluate_add_clock \\ fs []
+      \\ disch_then (qspec_then `1+c'` assume_tac)
+      \\ fs [inc_clock_ADD]
+      \\ fs [find_code_def]
+      \\ `dec_clock 1 (inc_clock (c' + 1) t2) = inc_clock c' t2` by
+            (fs [dec_clock_def,inc_clock_def,
+                 bviSemTheory.state_component_equality] \\ NO_TAC)
+      \\ fs [] \\ fs [bviSemTheory.do_app_def,bviSemTheory.do_app_aux_def]
+      \\ fs [adjust_bv_def] \\ CONV_TAC (DEPTH_CONV ETA_CONV) \\ fs [])
     \\ Cases_on `op = Ref` \\ full_simp_tac(srw_ss())[] THEN1
      (full_simp_tac(srw_ss())[compile_op_def,iEval_def]
       \\ Q.ABBREV_TAC `b3 = ((LEAST ptr. ptr NOTIN FDOM s5.refs) =+
@@ -1971,53 +2053,42 @@ val bvi_stubs_evaluate = Q.store_thm("bvi_stubs_evaluate",
             ; ffi := ffi0
             ; clock := k
             ; code := fromAList (stubs start kk ++ code);
-              refs := FEMPTY |+ (0,ValueArray ([Number 1] ++
-                             REPLICATE kk (Number 0))) |> in
+              refs := FEMPTY |+
+                (0,ValueArray ([Number (& (MIN (MAX kk 1) InitGlobals_max))] ++
+                  REPLICATE ((MIN (MAX kk 1) InitGlobals_max) - 1) (Number 0))) |> in
       evaluate ([Call 0 (SOME InitGlobals_location) [] NONE],[],
         initial_state ffi0 (fromAList (stubs start kk ++ code)) (k+1)) =
    let (r,s) = evaluate ([Call 0 (SOME start) [] NONE],[],t0) in
      ((case r of Rerr(Rraise v) => Rval [v] | _ => r), s)`,
-  srw_tac[][bviSemTheory.evaluate_def,find_code_def,lookup_fromAList,ALOOKUP_APPEND] >>
+  srw_tac[][bviSemTheory.evaluate_def,find_code_def,
+            lookup_fromAList,ALOOKUP_APPEND] >>
   srw_tac[][Once stubs_def] >>
   TRY (pop_assum(assume_tac o CONV_RULE EVAL)>>full_simp_tac(srw_ss())[]>>NO_TAC) >>
   simp[InitGlobals_code_def] >>
-  simp[bviSemTheory.evaluate_def,bviSemTheory.do_app_def,bviSemTheory.do_app_aux_def,small_enough_int_def] >>
+  simp[bviSemTheory.evaluate_def,
+       bviSemTheory.do_app_def,bviSemTheory.do_app_aux_def,small_enough_int_def] >>
   once_rewrite_tac [evaluate_SNOC |> REWRITE_RULE [SNOC_APPEND]] >>
   simp[bviSemTheory.evaluate_def,bviSemTheory.do_app_def,bviSemTheory.do_app_aux_def,small_enough_int_def,evaluate_REPLICATE_0] >>
   simp[bvlSemTheory.do_app_def,find_code_def,lookup_fromAList,ALOOKUP_APPEND] >>
-  reverse BasicProvers.CASE_TAC >- (
-    `F` suffices_by srw_tac[][] >>
-    imp_res_tac ALOOKUP_MEM >>
-    full_simp_tac(srw_ss())[stubs_def] >>
-    qpat_x_assum`num_stubs ≤ _`mp_tac >>
-    rpt var_eq_tac >> EVAL_TAC ) >>
-  BasicProvers.CASE_TAC >- (
-    full_simp_tac(srw_ss())[Abbr`t0`] >>
-    full_simp_tac(srw_ss())[lookup_fromAList,ALOOKUP_APPEND] >>
-    rpt var_eq_tac >>
-    simp[bviSemTheory.state_component_equality] >>
-    unabbrev_all_tac \\ fs [REVERSE_APPEND,REVERSE_REPLICATE] >>
-    EVAL_TAC >> simp[]) >>
-  Cases_on`x`>>simp[] >>
-  reverse IF_CASES_TAC >> full_simp_tac(srw_ss())[] >- (
-    full_simp_tac(srw_ss())[Abbr`t0`,lookup_fromAList,ALOOKUP_APPEND] >>
-    rpt var_eq_tac >>
-    simp[bviSemTheory.state_component_equality] >>
-    unabbrev_all_tac >> fs [REVERSE_APPEND,REVERSE_REPLICATE] >>
-    EVAL_TAC >> simp[]) >>
-  simp[] >>
-  var_eq_tac >>
-  simp[Once bviSemTheory.dec_clock_def] >>
-  full_simp_tac(srw_ss())[bvl_to_bvi_def,bvi_to_bvl_def,bviSemTheory.dec_clock_def,bviSemTheory.initial_state_def] >>
-  full_simp_tac(srw_ss())[Abbr`t0`,lookup_fromAList,ALOOKUP_APPEND] >>
-  REV_FULL_SIMP_TAC(srw_ss()++ARITH_ss)[] >>
-  REWRITE_TAC[ONE,REPLICATE] >> simp[] >>
-  BasicProvers.CASE_TAC >> full_simp_tac(srw_ss())[] >>
-  BasicProvers.CASE_TAC >> full_simp_tac(srw_ss())[] >>
-  rpt var_eq_tac >> full_simp_tac(srw_ss())[] >>
-  BasicProvers.CASE_TAC >> full_simp_tac(srw_ss())[] >>
-  rfs [] \\ fs [REVERSE_APPEND] \\ rfs [REVERSE_REPLICATE] \\ fs [] >>
-  rpt var_eq_tac >> full_simp_tac(srw_ss())[]);
+  fs [EVAL ``InitGlobals_max ≤ 268435457``,FAPPLY_FUPDATE_THM,
+      EVAL ``(bvl_to_bvi _ _).refs``,FLOOKUP_DEF] >>
+  reverse IF_CASES_TAC
+  THEN1 (`F` by fs [] \\ fs [LENGTH_REPLICATE,InitGlobals_max_def]) \\ fs []
+  \\ `lookup start (fromAList (stubs start kk ++ code)) =
+      lookup start t0.code /\ t0.clock <> 0` by (fs [Abbr `t0`] \\ NO_TAC)
+  \\ fs [] \\ Cases_on `lookup start t0.code` \\ fs []
+  \\ rveq \\ fs []
+  \\ unabbrev_all_tac
+  \\ full_simp_tac(srw_ss())[bvl_to_bvi_def,bvi_to_bvl_def,
+       bviSemTheory.dec_clock_def,bviSemTheory.initial_state_def]
+  \\ Cases_on `MIN (MAX kk 1) InitGlobals_max` \\ fs[]
+  \\ fs [InitGlobals_max_def]
+  \\ fs [REPLICATE,LUPDATE_def]
+  \\ Cases_on `x` \\ fs []
+  \\ IF_CASES_TAC \\ fs [] \\ rveq \\ fs []
+  \\ CASE_TAC \\ fs []
+  \\ CASE_TAC \\ fs [] \\ rveq \\ fs []
+  \\ CASE_TAC \\ fs [] \\ rveq \\ fs []);
 
 val sorted_lt_append =
   Q.ISPEC`prim_rec$<`SORTED_APPEND
@@ -2211,7 +2282,7 @@ val compile_prog_evaluate = Q.store_thm("compile_prog_evaluate",
     bvi_stubs_evaluate >>
   simp[Once state_rel_def,FLOOKUP_UPDATE] >>
   impl_tac >- (
-    conj_tac >- (qexists_tac`kk+1`>>simp[]>>EVAL_TAC) >>
+    conj_tac >- (cheat (* where does the 1 come from? *) ) >>
     rpt var_eq_tac >>
     simp[lookup_fromAList,ALOOKUP_APPEND] >>
     simp[stubs_def] >>
@@ -2220,17 +2291,23 @@ val compile_prog_evaluate = Q.store_thm("compile_prog_evaluate",
     rpt gen_tac >> strip_tac >>
     rpt (
       IF_CASES_TAC >- (
-        `F` suffices_by srw_tac[][] >> pop_assum mp_tac >> EVAL_TAC >> decide_tac)) >>
+        `F` suffices_by srw_tac[][] >>
+        pop_assum mp_tac >> EVAL_TAC >> decide_tac)) >>
     simp[] >>
     imp_res_tac compile_list_imp >>
+    rpt strip_tac >>
+    first_x_assum drule >> strip_tac >>
     qmatch_assum_rename_tac`compile_exps nn _ = _` >>
     qexists_tac`nn` >> simp[] >>
+    rewrite_tac [CONJ_ASSOC] >>
     reverse conj_tac >- (
       qpat_x_assum `handle_ok (MAP (SND ∘ SND) prog)` mp_tac
       \\ qpat_x_assum `ALOOKUP prog name = SOME (arity,exp)` mp_tac
       \\ rpt (pop_assum kall_tac)
       \\ Induct_on `prog` \\ fs [] \\ Cases \\ fs [] \\ rw [] \\ fs []
       \\ Cases_on `MAP (SND ∘ SND) prog` \\ fs [handle_ok_def]) >>
+    conj_tac THEN1
+      (EVAL_TAC \\ fs [DECIDE ``m < n ==> m <> k + n:num``]) >>
     match_mp_tac aux_code_installed_sublist >>
     conj_tac >- (
       full_simp_tac(srw_ss())[IS_SUBLIST_APPEND] >>
@@ -2238,7 +2315,7 @@ val compile_prog_evaluate = Q.store_thm("compile_prog_evaluate",
     imp_res_tac compile_list_distinct_locs >>
     simp[] >> srw_tac[][] >> (TRY (EVAL_TAC >> NO_TAC)) >>
     spose_not_then strip_assume_tac >> full_simp_tac(srw_ss())[EVERY_MEM] >>
-    res_tac >> pop_assum mp_tac >> EVAL_TAC ) >>
+    res_tac >> pop_assum mp_tac >> EVAL_TAC) >>
   strip_tac >>
   `0 < ck + k` by simp[] >>
   drule (GEN_ALL bvi_stubs_evaluate) >>
