compiler/backend/semantics/bviSemScript.sml
@@ -53,6 +53,15 @@ val do_app_aux_def = Define `
         (case xs of
          | [RefPtr p] => SOME (SOME (Unit, s with global := SOME p))
          | _ => NONE)
+    | (FromList n, xs) =>
+        (case xs of
+         | [len;lv] =>
+            (case v_to_list lv of
+             | SOME vs => if len = Number (& (LENGTH vs))
+                          then SOME (SOME (Block n vs, s))
+                          else SOME NONE
+             | _ => SOME NONE)
+         | _ => SOME NONE)
     | (Global n, _) => NONE
     | (SetGlobal n, _) => NONE
     | (AllocGlobal, _) => NONE
